sparse/spec_build_csr2.v
@@ -1,6 +1,6 @@
 Require Import VST.floyd.proofauto.
 Require Import Iterative.floatlib.
-From Iterative.sparse Require Import sparse_model build_csr2 distinct.
+From Iterative.sparse Require Import sparse_model build_csr2 distinct partial_csrg.
 Require Import vcfloat.FPStdCompCert.
 Require Import vcfloat.FPStdLib.
 Require Import VSTlib.spec_math VSTlib.spec_malloc.
@@ -15,12 +15,6 @@ Open Scope logic.
 
 #[export] Declare Instance M: MallocAPD.
 
-Check data_at.
-
-Compute reptype (Tarray (Tstruct  _rowcol noattr) 10 noattr).
-
-Print coo_matrix_wellformed.
-Print int.
 
 Definition intpair_to_valpair (a : int * int) : val * val :=
   match a with 
@@ -48,8 +42,8 @@ Definition swap_spec :=
     SEP (data_at sh (Tarray (Tstruct _rowcol noattr) (Zlength coog) noattr) (map intpair_to_valpair (upd_Znth a (upd_Znth b coog (Znth a coog)) (Znth b coog))) p).
 
 (* compare with the one in the repo that's verified *)
-Definition coo_quicksort_spec :=
- DECLARE _coo_quicksort
+Definition coog_quicksort_spec :=
+ DECLARE _coog_quicksort
  WITH sh: share, coog: list (int * int), p: val, base: Z, n: Z
  PRE [ tptr (Tstruct _rowcol noattr), tuint, tuint ]
     PROP(writable_share sh;
@@ -64,8 +58,8 @@ Definition coo_quicksort_spec :=
     RETURN( )
     SEP (data_at sh (Tarray (Tstruct  _rowcol noattr) (Zlength coog) noattr) (map intpair_to_valpair coog') p).
 
-Definition coo_count_spec :=
- DECLARE _coo_count
+Definition coog_count_spec :=
+ DECLARE _coog_count
  WITH sh: share, coog: list (int * int), p: val
  PRE [ tptr (Tstruct _rowcol noattr) ]
     PROP(writable_share sh;
@@ -78,8 +72,8 @@ Definition coo_count_spec :=
     RETURN( Vint (Int.repr (count_distinct (map intpair_to_Zpair coog))) )
     SEP (data_at sh (Tarray (Tstruct _rowcol noattr) (Zlength coog) noattr) (map intpair_to_valpair coog) p).
 
-Definition start_coo_shell_spec :=
-  DECLARE _start_coo_shell
+Definition start_coog_spec :=
+  DECLARE _start_coog
   WITH sh : share, n : int 
   PRE [tuint]
     PROP ()
@@ -92,8 +86,8 @@ Definition start_coo_shell_spec :=
     SEP (data_at_ sh (Tarray (Tstruct _rowcol noattr) (Int.intval n) noattr) p)
     .
 
-Definition add_to_coo_shell_spec :=
-  DECLARE _add_to_coo_shell 
+Definition add_to_coog_spec :=
+  DECLARE _add_to_coog
   WITH sh : share, coog : list (int * int), p : val, r : int, c : int, n : Z
   PRE [tptr (Tstruct _rowcol noattr), tuint, tuint, tuint]
     PROP ()
@@ -132,6 +126,7 @@ Definition csr_token (m: matrix Tdouble) (p: val) : mpred :=
  EX (csr: csr_matrix Tdouble) (H: csr_to_matrix csr m), csr_token' csr p.
 
 (* Just copied here so that I don't have to compile everything *)
+(*
 Definition coog_upto (i : Z) (coog : coog_matrix) :=
   Build_coog_matrix (coog_rows coog) (coog_cols coog) (sublist 0 i (coog_entries coog)).
 
@@ -159,10 +154,10 @@ Inductive coog_csr {t} (coog : coog_matrix) (csr : csr_matrix t) : Prop :=
     (coog_csr_vals : Zlength (csr_vals csr) = count_distinct (coog_entries coog))
     (coog_csr_entries : entries_correspond_coog coog csr)
     (coog_csr_zeros : no_extra_zeros_coog coog csr),
-    coog_csr coog csr.
+    coog_csr coog csr. *)
 (* End of copied code *)
 
-Definition coo_shell_to_csr_shell_spec :=
+Definition coog_to_csrg_spec :=
   DECLARE _coo_shell_to_csr_shell
   WITH sh : share, coog : list (int * int), p : val, rows : int, cols : int, gv : globals
   PRE [tptr (Tstruct _rowcol noattr), tuint, tuint, tuint]
@@ -180,3 +175,23 @@ Definition coo_shell_to_csr_shell_spec :=
     SEP (data_at sh (Tarray (Tstruct _rowcol noattr) (Zlength coog) noattr) (map intpair_to_valpair coog') p;
       csr_rep Ews csr q;
       mem_mgr gv).
+
+Definition surely_malloc_spec :=
+  DECLARE _surely_malloc
+   WITH t:Ctypes.type, gv: globals
+   PRE [ size_t ]
+       PROP (0 <= sizeof t <= Ptrofs.max_unsigned;
+                complete_legal_cosu_type t = true;
+                natural_aligned natural_alignment t = true)
+       PARAMS (Vptrofs (Ptrofs.repr (sizeof t))) GLOBALS (gv)
+       SEP (mem_mgr gv)
+    POST [ tptr tvoid ] EX p:_,
+       PROP ()
+       LOCAL (temp ret_temp p)
+       SEP (mem_mgr gv; malloc_token Ews t p * data_at_ Ews t p).
+
+Definition Build_CSR2_ASI : funspecs := [
+  surely_malloc_spec; swap_spec; coog_quicksort_spec; 
+  coog_count_spec; start_coog_spec; add_to_coog_spec;
+  coog_to_csrg_spec
+].
